Wrote up unstructuring

11UnstructuredState/UnstructuredState.thy
@@ -15,8 +15,8 @@ code-pointer, because the code-pointer is referenced in every single operation. 
 tail of the callstack into the memory map, and keep the head (which is the current code pointer) in
 its own register.\<close>
 
-datatype unstr_state = 
-  S\<^sub>u "nat \<Rightarrow> pointer_tag \<times> nat" nat "nat \<Rightarrow> nat" nat "nat \<Rightarrow> nat" nat "nat \<Rightarrow> nat" nat nat
+datatype state\<^sub>r = 
+  S\<^sub>r "nat \<Rightarrow> pointer_tag \<times> nat" nat "nat \<Rightarrow> nat" nat "nat \<Rightarrow> nat" nat "nat \<Rightarrow> nat" nat nat
 
 fun unstr_lookup :: "(nat \<Rightarrow> nat) \<Rightarrow> nat \<Rightarrow> nat \<rightharpoonup> nat" where
   "unstr_lookup h 0 x = None"
@@ -24,51 +24,50 @@ fun unstr_lookup :: "(nat \<Rightarrow> nat) \<Rightarrow> nat \<Rightarrow> nat
 | "unstr_lookup h (Suc (Suc p)) 0 = (if even p then Some (h p) else None)"
 | "unstr_lookup h (Suc (Suc p)) (Suc x) = (if even p then unstr_lookup h (h (Suc p)) x else None)"
 
-inductive eval\<^sub>u :: "code\<^sub>b list \<Rightarrow> unstr_state \<Rightarrow> unstr_state \<Rightarrow> bool" (infix "\<tturnstile> _ \<leadsto>\<^sub>u" 50) where
-  ev\<^sub>u_lookup [simp]: "lookup \<C> p\<^sub>\<C> = Some (Lookup\<^sub>b x) \<Longrightarrow> unstr_lookup \<Delta> (s p\<^sub>s) x = Some y \<Longrightarrow>
-    \<C> \<tturnstile> S\<^sub>u h p\<^sub>h \<Delta> p\<^sub>\<Delta> \<V> p\<^sub>\<V> s (Suc p\<^sub>s) (Suc p\<^sub>\<C>) \<leadsto>\<^sub>u S\<^sub>u h p\<^sub>h \<Delta> p\<^sub>\<Delta> (\<V>(p\<^sub>\<V> := y)) (Suc p\<^sub>\<V>) s (Suc p\<^sub>s) p\<^sub>\<C>"
-| ev\<^sub>u_pushcon [simp]: "lookup \<C> p\<^sub>\<C> = Some (PushCon\<^sub>b n) \<Longrightarrow> 
-    \<C> \<tturnstile> S\<^sub>u h p\<^sub>h \<Delta> p\<^sub>\<Delta> \<V> p\<^sub>\<V> s (Suc p\<^sub>s) (Suc p\<^sub>\<C>) \<leadsto>\<^sub>u 
-      S\<^sub>u (h(p\<^sub>h := (PConst, n), Suc p\<^sub>h := (PConst, 0))) (2 + p\<^sub>h) \<Delta> p\<^sub>\<Delta> 
-        (\<V>(p\<^sub>\<V> := p\<^sub>h)) (Suc p\<^sub>\<V>) s (Suc p\<^sub>s) p\<^sub>\<C>"
-| ev\<^sub>u_pushlam [simp]: "lookup \<C> p\<^sub>\<C> = Some (PushLam\<^sub>b p\<^sub>\<C>') \<Longrightarrow> 
-    \<C> \<tturnstile> S\<^sub>u h p\<^sub>h \<Delta> p\<^sub>\<Delta> \<V> p\<^sub>\<V> s (Suc p\<^sub>s) (Suc p\<^sub>\<C>) \<leadsto>\<^sub>u 
-      S\<^sub>u (h(p\<^sub>h := (PEnv, s p\<^sub>s), Suc p\<^sub>h := (PCode, p\<^sub>\<C>'))) (2 + p\<^sub>h) \<Delta> p\<^sub>\<Delta> 
-        (\<V>(p\<^sub>\<V> := p\<^sub>h)) (Suc p\<^sub>\<V>) s (Suc p\<^sub>s) p\<^sub>\<C>"
-| ev\<^sub>u_apply [simp]: "lookup \<C> p\<^sub>\<C> = Some Apply\<^sub>b \<Longrightarrow> h (\<V> p\<^sub>\<V>) = (PEnv, p\<^sub>\<Delta>') \<Longrightarrow> 
-    h (Suc (\<V> p\<^sub>\<V>)) = (PCode, p\<^sub>\<C>') \<Longrightarrow>
-    \<C> \<tturnstile> S\<^sub>u h p\<^sub>h \<Delta> p\<^sub>\<Delta> \<V> (Suc (Suc p\<^sub>\<V>)) s (Suc p\<^sub>s) (Suc p\<^sub>\<C>) \<leadsto>\<^sub>u 
-      S\<^sub>u h p\<^sub>h (\<Delta>(p\<^sub>\<Delta> := \<V> (Suc p\<^sub>\<V>), Suc p\<^sub>\<Delta> := p\<^sub>\<Delta>')) (2 + p\<^sub>\<Delta>) \<V> p\<^sub>\<V>
-        (s(Suc p\<^sub>s := p\<^sub>\<C>, Suc (Suc p\<^sub>s) := Suc (Suc p\<^sub>\<Delta>))) (2 + Suc p\<^sub>s) p\<^sub>\<C>'"
-| ev\<^sub>u_return [simp]: "lookup \<C> p\<^sub>\<C> = Some Return\<^sub>b \<Longrightarrow> 
-    \<C> \<tturnstile> S\<^sub>u h p\<^sub>h \<Delta> p\<^sub>\<Delta> \<V> p\<^sub>\<V> s (Suc (Suc p\<^sub>s)) (Suc p\<^sub>\<C>) \<leadsto>\<^sub>u 
-      S\<^sub>u h p\<^sub>h \<Delta> p\<^sub>\<Delta> \<V> p\<^sub>\<V> s p\<^sub>s (s p\<^sub>s)"
-| ev\<^sub>u_jump [simp]: "lookup \<C> p\<^sub>\<C> = Some Jump\<^sub>b \<Longrightarrow> h (\<V> p\<^sub>\<V>) = (PEnv, p\<^sub>\<Delta>') \<Longrightarrow> 
-    h (Suc (\<V> p\<^sub>\<V>)) = (PCode, p\<^sub>\<C>') \<Longrightarrow> 
-    \<C> \<tturnstile> S\<^sub>u h p\<^sub>h \<Delta> p\<^sub>\<Delta> \<V> (Suc (Suc p\<^sub>\<V>)) s (Suc p\<^sub>s) (Suc p\<^sub>\<C>) \<leadsto>\<^sub>u 
-      S\<^sub>u h p\<^sub>h (\<Delta>(p\<^sub>\<Delta> := \<V> (Suc p\<^sub>\<V>), Suc p\<^sub>\<Delta> := p\<^sub>\<Delta>')) (2 + p\<^sub>\<Delta>) \<V> p\<^sub>\<V>
-        (s(p\<^sub>s := Suc (Suc p\<^sub>\<Delta>))) (Suc p\<^sub>s) p\<^sub>\<C>'"
+inductive eval\<^sub>r :: "code\<^sub>b list \<Rightarrow> state\<^sub>r \<Rightarrow> state\<^sub>r \<Rightarrow> bool" (infix "\<tturnstile> _ \<leadsto>\<^sub>r" 50) where
+  ev\<^sub>r_lookup [simp]: "lookup \<C> p\<^sub>\<C> = Some (Lookup\<^sub>b x) \<Longrightarrow> unstr_lookup \<Delta> (s b\<^sub>s) x = Some y \<Longrightarrow>
+    \<C> \<tturnstile> S\<^sub>r h b\<^sub>h \<Delta> b\<^sub>\<Delta> \<V> b\<^sub>\<V> s (Suc b\<^sub>s) (Suc p\<^sub>\<C>) \<leadsto>\<^sub>r S\<^sub>r h b\<^sub>h \<Delta> b\<^sub>\<Delta> (\<V>(b\<^sub>\<V> := y)) (Suc b\<^sub>\<V>) s (Suc b\<^sub>s) p\<^sub>\<C>"
+| ev\<^sub>r_pushcon [simp]: "lookup \<C> p\<^sub>\<C> = Some (PushCon\<^sub>b n) \<Longrightarrow> 
+    \<C> \<tturnstile> S\<^sub>r h b\<^sub>h \<Delta> b\<^sub>\<Delta> \<V> b\<^sub>\<V> s (Suc b\<^sub>s) (Suc p\<^sub>\<C>) \<leadsto>\<^sub>r 
+      S\<^sub>r (h(b\<^sub>h := (PConst, n), Suc b\<^sub>h := (PConst, 0))) (2 + b\<^sub>h) \<Delta> b\<^sub>\<Delta> (\<V>(b\<^sub>\<V> := b\<^sub>h)) (Suc b\<^sub>\<V>) s 
+        (Suc b\<^sub>s) p\<^sub>\<C>"
+| ev\<^sub>r_pushlam [simp]: "lookup \<C> p\<^sub>\<C> = Some (PushLam\<^sub>b p\<^sub>\<C>') \<Longrightarrow> 
+    \<C> \<tturnstile> S\<^sub>r h b\<^sub>h \<Delta> b\<^sub>\<Delta> \<V> b\<^sub>\<V> s (Suc b\<^sub>s) (Suc p\<^sub>\<C>) \<leadsto>\<^sub>r 
+      S\<^sub>r (h(b\<^sub>h := (PEnv, s b\<^sub>s), Suc b\<^sub>h := (PCode, p\<^sub>\<C>'))) (2 + b\<^sub>h) \<Delta> b\<^sub>\<Delta> (\<V>(b\<^sub>\<V> := b\<^sub>h)) (Suc b\<^sub>\<V>) s 
+        (Suc b\<^sub>s) p\<^sub>\<C>"
+| ev\<^sub>r_apply [simp]: "lookup \<C> p\<^sub>\<C> = Some Apply\<^sub>b \<Longrightarrow> h (\<V> b\<^sub>\<V>) = (PEnv, p\<^sub>\<Delta>) \<Longrightarrow> 
+    h (Suc (\<V> b\<^sub>\<V>)) = (PCode, p\<^sub>\<C>') \<Longrightarrow>
+    \<C> \<tturnstile> S\<^sub>r h b\<^sub>h \<Delta> b\<^sub>\<Delta> \<V> (Suc (Suc b\<^sub>\<V>)) s (Suc b\<^sub>s) (Suc p\<^sub>\<C>) \<leadsto>\<^sub>r 
+      S\<^sub>r h b\<^sub>h (\<Delta>(b\<^sub>\<Delta> := \<V> (Suc b\<^sub>\<V>), Suc b\<^sub>\<Delta> := p\<^sub>\<Delta>)) (2 + b\<^sub>\<Delta>) \<V> b\<^sub>\<V>
+        (s(Suc b\<^sub>s := p\<^sub>\<C>, Suc (Suc b\<^sub>s) := Suc (Suc b\<^sub>\<Delta>))) (2 + Suc b\<^sub>s) p\<^sub>\<C>'"
+| ev\<^sub>r_return [simp]: "lookup \<C> p\<^sub>\<C> = Some Return\<^sub>b \<Longrightarrow> 
+    \<C> \<tturnstile> S\<^sub>r h b\<^sub>h \<Delta> b\<^sub>\<Delta> \<V> b\<^sub>\<V> s (Suc (Suc b\<^sub>s)) (Suc p\<^sub>\<C>) \<leadsto>\<^sub>r S\<^sub>r h b\<^sub>h \<Delta> b\<^sub>\<Delta> \<V> b\<^sub>\<V> s b\<^sub>s (s b\<^sub>s)"
+| ev\<^sub>r_jump [simp]: "lookup \<C> p\<^sub>\<C> = Some Jump\<^sub>b \<Longrightarrow> h (\<V> b\<^sub>\<V>) = (PEnv, p\<^sub>\<Delta>) \<Longrightarrow> 
+    h (Suc (\<V> b\<^sub>\<V>)) = (PCode, p\<^sub>\<C>') \<Longrightarrow> 
+    \<C> \<tturnstile> S\<^sub>r h b\<^sub>h \<Delta> b\<^sub>\<Delta> \<V> (Suc (Suc b\<^sub>\<V>)) s (Suc b\<^sub>s) (Suc p\<^sub>\<C>) \<leadsto>\<^sub>r 
+      S\<^sub>r h b\<^sub>h (\<Delta>(b\<^sub>\<Delta> := \<V> (Suc b\<^sub>\<V>), Suc b\<^sub>\<Delta> := p\<^sub>\<Delta>)) (2 + b\<^sub>\<Delta>) \<V> b\<^sub>\<V> (s(b\<^sub>s := Suc (Suc b\<^sub>\<Delta>))) 
+        (Suc b\<^sub>s) p\<^sub>\<C>'"
 
-theorem determinismu: "\<C> \<tturnstile> \<Sigma> \<leadsto>\<^sub>u \<Sigma>' \<Longrightarrow> \<C> \<tturnstile> \<Sigma> \<leadsto>\<^sub>u \<Sigma>'' \<Longrightarrow> \<Sigma>' = \<Sigma>''"
-proof (induction \<C> \<Sigma> \<Sigma>' rule: eval\<^sub>u.induct)
-  case ev\<^sub>u_lookup
-  from ev\<^sub>u_lookup(3, 1, 2) show ?case by (induction rule: eval\<^sub>u.cases) simp_all
+theorem determinism\<^sub>r: "\<C> \<tturnstile> \<Sigma> \<leadsto>\<^sub>r \<Sigma>' \<Longrightarrow> \<C> \<tturnstile> \<Sigma> \<leadsto>\<^sub>r \<Sigma>'' \<Longrightarrow> \<Sigma>' = \<Sigma>''"
+proof (induction \<C> \<Sigma> \<Sigma>' rule: eval\<^sub>r.induct)
+  case ev\<^sub>r_lookup
+  from ev\<^sub>r_lookup(3, 1, 2) show ?case by (induction rule: eval\<^sub>r.cases) simp_all
 next
 next
-  case ev\<^sub>u_pushcon
-  from ev\<^sub>u_pushcon(2, 1) show ?case by (induction rule: eval\<^sub>u.cases) simp_all
+  case ev\<^sub>r_pushcon
+  from ev\<^sub>r_pushcon(2, 1) show ?case by (induction rule: eval\<^sub>r.cases) simp_all
 next
-  case ev\<^sub>u_pushlam
-  from ev\<^sub>u_pushlam(2, 1) show ?case by (induction rule: eval\<^sub>u.cases) simp_all
+  case ev\<^sub>r_pushlam
+  from ev\<^sub>r_pushlam(2, 1) show ?case by (induction rule: eval\<^sub>r.cases) simp_all
 next
-  case ev\<^sub>u_apply
-  from ev\<^sub>u_apply(4, 1, 2, 3) show ?case by (induction rule: eval\<^sub>u.cases) simp_all
+  case ev\<^sub>r_apply
+  from ev\<^sub>r_apply(4, 1, 2, 3) show ?case by (induction rule: eval\<^sub>r.cases) simp_all
 next
-  case ev\<^sub>u_return
-  from ev\<^sub>u_return(2, 1) show ?case by (induction rule: eval\<^sub>u.cases) simp_all
+  case ev\<^sub>r_return
+  from ev\<^sub>r_return(2, 1) show ?case by (induction rule: eval\<^sub>r.cases) simp_all
 next
-  case ev\<^sub>u_jump
-  from ev\<^sub>u_jump(4, 1, 2, 3) show ?case by (induction rule: eval\<^sub>u.cases) simp_all
+  case ev\<^sub>r_jump
+  from ev\<^sub>r_jump(4, 1, 2, 3) show ?case by (induction rule: eval\<^sub>r.cases) simp_all
 qed
 
 end
