Readme.md
@@ -6,7 +6,6 @@ Goals:
 - do reverse of type-saftey for conversions
 - Do reverse proofs for typechecking, assembly, machine?
 - Modularize code with classes
-- Remove runtime tags (need tags for code pointers in late stages)
 - Add Parser?
 - Add pairs, sums, unit, void, nats, primrec? sructured types?
 - Make printing part of the code
@@ -20,3 +19,4 @@ Refactorings:
 - rename closure stuff
 - Make late stage closures (post bytecode) a single parametric datatype?
 - Clean up isabelle - declare x.simps[intros], assumes/shows, patterns in pfs
+- Use ints insted of nats for machine code
